src/ProbabilisticProgramming/Loops.dfy
@@ -13,81 +13,10 @@ module Loops {
    Definitions
   ************/
 
-  // Definition 37
-  function WhileCut<A>(condition: A -> bool, body: A -> Monad.Hurd<A>, init: A, fuel: nat): Monad.Hurd<A> {
-    if fuel == 0 || !condition(init) then
-      Monad.Return(init)
-    else
-      Monad.Bind(body(init), (init': A) => WhileCut(condition, body, init', fuel - 1))
-  }
-
-  ghost predicate WhileCutTerminates<A>(condition: A -> bool, body: A -> Monad.Hurd<A>, init: A, s: Rand.Bitstream) {
-    exists fuel: nat :: WhileCutTerminatesWithFuel(condition, body, init, s)(fuel)
-  }
-
-  ghost function WhileCutTerminatesWithFuel<A>(condition: A -> bool, body: A -> Monad.Hurd<A>, init: A, s: Rand.Bitstream): nat -> bool {
-    (fuel: nat) => !WhileCut(condition, body, init, fuel)(s).Satisfies(condition)
-  }
-
-  // Definition 39 / True iff Prob(iset s | While(condition, body, a)(s) terminates) == 1
-  ghost predicate WhileTerminatesAlmostSurely<A(!new)>(condition: A -> bool, body: A -> Monad.Hurd<A>) {
-    var p := (init: A) =>
-               (s: Rand.Bitstream) => WhileCutTerminates(condition, body, init, s);
-    forall init :: Quantifier.AlmostSurely(p(init))
-  }
-
-  // Definition of while loops.
-  // This definition is opaque because the details are not very useful.
-  // For proofs, use the lemma `WhileUnroll`.
-  // Equation (3.25), but modified to use `Monad.Diverging` instead of HOL's `arb` in case of nontermination
-  opaque ghost function While<A(!new)>(condition: A -> bool, body: A -> Monad.Hurd<A>): (loop: A -> Monad.Hurd<A>)
-    ensures forall s: Rand.Bitstream, init: A :: !condition(init) ==> loop(init)(s) == Monad.Return(init)(s)
-  {
-    var f :=
-      (init: A) =>
-        (s: Rand.Bitstream) =>
-          if WhileCutTerminates(condition, body, init, s)
-          then
-            var fuel := LeastFuel(condition, body, init, s);
-            WhileCut(condition, body, init, fuel)(s)
-          else
-            Monad.Diverging;
-    assert forall s: Rand.Bitstream, init: A :: !condition(init) ==> f(init)(s) == Monad.Return(init)(s) by {
-      forall s: Rand.Bitstream, init: A ensures !condition(init) ==> f(init)(s) == Monad.Return(init)(s) {
-        if !condition(init) {
-          assert WhileCutTerminatesWithFuel(condition, body, init, s)(0);
-        }
-      }
-    }
-    f
-  }
-
-  ghost function LeastFuel<A>(condition: A -> bool, body: A -> Monad.Hurd<A>, init: A, s: Rand.Bitstream): (fuel: nat)
-    requires WhileCutTerminates(condition, body, init, s)
-    ensures WhileCutTerminatesWithFuel(condition, body, init, s)(fuel)
-    ensures forall fuel': nat :: WhileCutTerminatesWithFuel(condition, body, init, s)(fuel') ==> fuel <= fuel'
-  {
-    var fuelBound :| WhileCutTerminatesWithFuel(condition, body, init, s)(fuelBound);
-    Least(WhileCutTerminatesWithFuel(condition, body, init, s), fuelBound)
-  }
-
-  ghost function Least(property: nat -> bool, bound: nat, start: nat := 0): (l: nat)
-    decreases bound - start
-    requires start <= bound
-    requires property(bound)
-    ensures property(l)
-    ensures start <= l <= bound
-    ensures forall n: nat | start <= n :: property(n) ==> l <= n
-  {
-    if start == bound || property(start)
-    then start
-    else Least(property, bound, start + 1)
-  }
-
   ghost predicate UntilTerminatesAlmostSurely<A(!new)>(proposal: Monad.Hurd<A>, accept: A -> bool) {
     var reject := (a: A) => !accept(a);
     var body := (a: A) => proposal;
-    WhileTerminatesAlmostSurely(reject, body)
+    Monad.WhileTerminatesAlmostSurely(reject, body)
   }
 
   // Definition of until loops (rejection sampling).
@@ -98,43 +27,43 @@ module Loops {
     ensures
       var reject := (a: A) => !accept(a);
       var body := (a: A) => proposal;
-      forall s :: f(s) == proposal(s).Bind(While(reject, body))
+      forall s :: Monad.Run(f)(s) == Monad.Run(proposal)(s).Bind(Monad.While(reject, body))
   {
     var reject := (a: A) => !accept(a);
     var body := (a: A) => proposal;
-    Monad.Bind(proposal, While(reject, body))
+    Monad.Bind(proposal, Monad.While(reject, body))
   }
 
   function WhileLoopExitsAfterOneIteration<A(!new)>(body: A -> Monad.Hurd<A>, condition: A -> bool, init: A): (Rand.Bitstream -> bool) {
     (s: Rand.Bitstream) =>
-      body(init)(s).Satisfies(v => !condition(v))
+      Monad.Run(body(init))(s).Satisfies(v => !condition(v))
   }
 
   function ProposalIsAccepted<A(!new)>(proposal: Monad.Hurd<A>, accept: A -> bool): (Rand.Bitstream -> bool) {
     (s: Rand.Bitstream) =>
-      proposal(s).Satisfies(accept)
+      Monad.Run(proposal)(s).Satisfies(accept)
   }
 
   ghost function UntilLoopResultIsAccepted<A(!new)>(proposal: Monad.Hurd<A>, accept: A -> bool): (Rand.Bitstream -> bool)
     requires UntilTerminatesAlmostSurely(proposal, accept)
   {
-    (s: Rand.Bitstream) => Until(proposal, accept)(s).Satisfies(accept)
+    (s: Rand.Bitstream) => Monad.Run(Until(proposal, accept))(s).Satisfies(accept)
   }
 
   ghost function UntilLoopResultHasProperty<A(!new)>(proposal: Monad.Hurd<A>, accept: A -> bool, property: A -> bool): iset<Rand.Bitstream>
     requires UntilTerminatesAlmostSurely(proposal, accept)
   {
-    iset s | Until(proposal, accept)(s).Satisfies(property)
+    iset s | Monad.Run(Until(proposal, accept))(s).Satisfies(property)
   }
 
   ghost function ProposalIsAcceptedAndHasProperty<A>(proposal: Monad.Hurd<A>, accept: A -> bool, property: A -> bool): iset<Rand.Bitstream>
   {
-    iset s | proposal(s).Satisfies(property) && proposal(s).Satisfies(accept)
+    iset s | Monad.Run(proposal)(s).Satisfies(property) && Monad.Run(proposal)(s).Satisfies(accept)
   }
 
   ghost function ProposalAcceptedEvent<A>(proposal: Monad.Hurd<A>, accept: A -> bool): iset<Rand.Bitstream>
   {
-    iset s | proposal(s).Satisfies(accept)
+    iset s | Monad.Run(proposal)(s).Satisfies(accept)
   }
 
 
@@ -142,157 +71,14 @@ module Loops {
    Lemmas
   *******/
 
-  lemma LeastFuelUnroll<A>(condition: A -> bool, body: A -> Monad.Hurd<A>, init: A, s: Rand.Bitstream, init': A, s': Rand.Bitstream, fuel': nat)
-    requires WhileCutTerminates(condition, body, init', s')
-    requires LeastFuel(condition, body, init', s') == fuel'
-    requires condition(init)
-    requires body(init)(s) == Monad.Result(init', s')
-    ensures WhileCutTerminates(condition, body, init, s)
-    ensures LeastFuel(condition, body, init, s) == fuel' + 1
-  {
-    assert WhileCutTerminates(condition, body, init, s) by {
-      WhileCutTerminatesWithFuelUnroll(condition, body, init, s, init', s', fuel');
-    }
-    var fuel := LeastFuel(condition, body, init, s);
-    assert fuel == fuel' + 1 by {
-      WhileCutTerminatesWithFuelUnroll(condition, body, init, s, init', s', fuel');
-      WhileCutTerminatesWithFuelUnroll(condition, body, init, s, init', s', fuel - 1);
-    }
-  }
-
-  lemma WhileCutUnroll<A>(condition: A -> bool, body: A -> Monad.Hurd<A>, init: A, s: Rand.Bitstream, init': A, s': Rand.Bitstream, fuel: nat)
-    requires condition(init)
-    requires body(init)(s) == Monad.Result(init', s')
-    ensures WhileCut(condition, body, init, fuel + 1)(s) == WhileCut(condition, body, init', fuel)(s')
-  {}
-
-
-  lemma WhileCutTerminatesWithFuelUnroll<A>(condition: A -> bool, body: A -> Monad.Hurd<A>, init: A, s: Rand.Bitstream, init': A, s': Rand.Bitstream, fuel: nat)
-    requires condition(init)
-    requires body(init)(s) == Monad.Result(init', s')
-    ensures WhileCutTerminatesWithFuel(condition, body, init, s)(fuel + 1) == WhileCutTerminatesWithFuel(condition, body, init', s')(fuel)
-  {}
-
-  lemma WhileCutTerminatesUnroll<A>(condition: A -> bool, body: A -> Monad.Hurd<A>, init: A, s: Rand.Bitstream, init': A, s': Rand.Bitstream)
-    requires condition(init)
-    requires body(init)(s) == Monad.Result(init', s')
-    ensures WhileCutTerminates(condition, body, init, s) == WhileCutTerminates(condition, body, init', s')
-  {
-    if WhileCutTerminates(condition, body, init, s) {
-      var fuel: nat :| WhileCutTerminatesWithFuel(condition, body, init, s)(fuel);
-      WhileCutTerminatesWithFuelUnroll(condition, body, init, s, init', s', fuel - 1);
-    }
-    if WhileCutTerminates(condition, body, init', s') {
-      var fuel: nat :| WhileCutTerminatesWithFuel(condition, body, init', s')(fuel);
-      WhileCutTerminatesWithFuelUnroll(condition, body, init, s, init', s', fuel);
-    }
-  }
-
-  lemma WhileUnrollIfConditionSatisfied<A>(condition: A -> bool, body: A -> Monad.Hurd<A>, init: A, s: Rand.Bitstream, init': A, s': Rand.Bitstream, loop: Monad.Result<A>, unrolled: Monad.Result<A>)
-    requires WhileCutTerminates(condition, body, init, s)
-    requires condition(init)
-    requires body(init)(s) == Monad.Result(init', s')
-    requires loop == While(condition, body)(init)(s)
-    requires unrolled == While(condition, body)(init')(s')
-    ensures loop == unrolled
-  {
-    var fuel: nat := LeastFuel(condition, body, init, s);
-    assert fuel >= 1;
-    var fuel': nat := fuel - 1;
-    assert WhileCutTerminatesWithFuel(condition, body, init', s')(fuel');
-    assert WhileCutTerminates(condition, body, init', s');
-    var minFuel: nat := LeastFuel(condition, body, init', s');
-    assert minFuel == fuel' by {
-      LeastFuelUnroll(condition, body, init, s, init', s', minFuel);
-    }
-    assert loop == unrolled by {
-      calc {
-        loop;
-        { reveal While(); }
-        WhileCut(condition, body, init, fuel)(s);
-        { WhileCutUnroll(condition, body, init, s, init', s', fuel'); }
-        WhileCut(condition, body, init', fuel')(s');
-        { reveal While(); }
-        unrolled;
-      }
-    }
-  }
-
-  lemma WhileUnrollIfTerminates<A(!new)>(condition: A -> bool, body: A -> Monad.Hurd<A>, init: A, s: Rand.Bitstream, fuel: nat, loop: Monad.Result<A>, unrolled: Monad.Result<A>)
-    requires WhileCutTerminates(condition, body, init, s)
-    requires fuel == LeastFuel(condition, body, init, s)
-    requires loop == While(condition, body)(init)(s)
-    requires unrolled == (if condition(init) then Monad.Bind(body(init), While(condition, body)) else Monad.Return(init))(s)
-    ensures loop == unrolled
-  {
-    if condition(init) {
-      assert fuel >= 1;
-      match body(init)(s)
-      case Diverging =>
-        calc {
-          loop;
-          { reveal While(); }
-          WhileCut(condition, body, init, fuel)(s);
-          Monad.Diverging;
-          unrolled;
-        }
-      case Result(init', s') =>
-        calc {
-          loop;
-          { WhileUnrollIfConditionSatisfied(condition, body, init, s, init', s', loop, unrolled); }
-          While(condition, body)(init')(s');
-          unrolled;
-        }
-    } else {
-      calc {
-        loop;
-        Monad.Result(init, s);
-        unrolled;
-      }
-    }
-  }
-
-  lemma WhileUnrollIfDiverges<A>(condition: A -> bool, body: A -> Monad.Hurd<A>, init: A, s: Rand.Bitstream, loop: Monad.Result<A>, unrolled: Monad.Result<A>)
-    requires !WhileCutTerminates(condition, body, init, s)
-    requires loop == While(condition, body)(init)(s)
-    requires unrolled == (if condition(init) then Monad.Bind(body(init), While(condition, body)) else Monad.Return(init))(s)
-    ensures loop == unrolled == Monad.Diverging
-  {
-    reveal While();
-    match body(init)(s)
-    case Diverging =>
-      assert unrolled == Monad.Diverging;
-    case Result(init', s') =>
-      assert !WhileCutTerminates(condition, body, init', s') by {
-        WhileCutTerminatesUnroll(condition, body, init, s, init', s');
-      }
-  }
-
-  // Theorem 38
-  lemma WhileUnroll<A(!new)>(condition: A -> bool, body: A -> Monad.Hurd<A>, init: A, s: Rand.Bitstream)
-    requires WhileTerminatesAlmostSurely(condition, body)
-    ensures While(condition, body)(init)(s) == (if condition(init) then Monad.Bind(body(init), While(condition, body)) else Monad.Return(init))(s)
-  {
-    var loop := While(condition, body)(init)(s);
-    var unrolled := (if condition(init) then Monad.Bind(body(init), While(condition, body)) else Monad.Return(init))(s);
-    assert loop == unrolled by {
-      if WhileCutTerminates(condition, body, init, s) {
-        var fuel: nat := LeastFuel(condition, body, init, s);
-        WhileUnrollIfTerminates(condition, body, init, s, fuel, loop, unrolled);
-      } else {
-        WhileUnrollIfDiverges(condition, body, init, s, loop, unrolled);
-      }
-    }
-  }
-
   lemma EnsureUntilTerminates<A(!new)>(proposal: Monad.Hurd<A>, accept: A -> bool)
     requires Independence.IsIndep(proposal)
-    requires Quantifier.WithPosProb((s: Rand.Bitstream) => proposal(s).Satisfies(accept))
+    requires Quantifier.WithPosProb((s: Rand.Bitstream) => Monad.Run(proposal)(s).Satisfies(accept))
     ensures UntilTerminatesAlmostSurely(proposal, accept)
   {
     var reject := (a: A) => !accept(a);
     var body := (a: A) => proposal;
-    var proposalIsAccepted := (s: Rand.Bitstream) => proposal(s).Satisfies(accept);
+    var proposalIsAccepted := (s: Rand.Bitstream) => Monad.Run(proposal)(s).Satisfies(accept);
     assert UntilTerminatesAlmostSurely(proposal, accept) by {
       forall a: A ensures Independence.IsIndep(body(a)) {
         assert body(a) == proposal;
@@ -301,7 +87,7 @@ module Loops {
         assert Quantifier.WithPosProb(proposalIsAccepted);
         assert (iset s | proposalIsAccepted(s)) == (iset s | WhileLoopExitsAfterOneIteration(body, reject, a)(s));
       }
-      assert WhileTerminatesAlmostSurely(reject, body) by {
+      assert Monad.WhileTerminatesAlmostSurely(reject, body) by {
         EnsureWhileTerminates(reject, body);
       }
     }
@@ -311,7 +97,7 @@ module Loops {
   lemma {:axiom} EnsureWhileTerminates<A(!new)>(condition: A -> bool, body: A -> Monad.Hurd<A>)
     requires forall a :: Independence.IsIndep(body(a))
     requires forall a :: Quantifier.WithPosProb(WhileLoopExitsAfterOneIteration(body, condition, a))
-    ensures WhileTerminatesAlmostSurely(condition, body)
+    ensures Monad.WhileTerminatesAlmostSurely(condition, body)
 
   // Theorem 45 (wrong!) / PROB_BERN_UNTIL (correct!)
   lemma {:axiom} UntilProbabilityFraction<A>(proposal: Monad.Hurd<A>, accept: A -> bool, d: A -> bool)
@@ -329,13 +115,17 @@ module Loops {
   lemma UntilUnroll<A(!new)>(proposal: Monad.Hurd<A>, accept: A -> bool, s: Rand.Bitstream)
     requires Independence.IsIndep(proposal)
     requires UntilTerminatesAlmostSurely(proposal, accept)
-    ensures Until(proposal, accept)(s) == Monad.Bind(proposal, (x: A) => if accept(x) then Monad.Return(x) else Until(proposal, accept))(s)
+    ensures Monad.Run(Until(proposal, accept))(s) == Monad.Run(Monad.Bind(proposal, (x: A) => if accept(x) then Monad.Return(x) else Until(proposal, accept)))(s)
   {
     var reject := (a: A) => !accept(a);
     var body := (a: A) => proposal;
-    match proposal(s)
+    match Monad.Run(proposal)(s)
     case Diverging =>
-    case Result(init, s') => WhileUnroll(reject, body, init, s');
+    case Result(init, s') => {
+      assert Monad.Run(Monad.While(reject, body)(init))(s') == Monad.Run(if reject(init) then Monad.Bind(body(init), Monad.While(reject, body)) else Monad.Return(init))(s') by {
+        Monad.WhileUnroll(reject, body, init, s');
+      }
+    }
   }
 
   // Equation (3.40)
@@ -351,22 +141,22 @@ module Loops {
 
   lemma WhileCutIsIndep<A(!new)>(condition: A -> bool, body: A -> Monad.Hurd<A>, init: A, fuel: nat)
     requires forall a: A :: Independence.IsIndep(body(a))
-    ensures Independence.IsIndep(WhileCut(condition, body, init, fuel))
+    ensures Independence.IsIndep(Monad.WhileCut(condition, body, init, fuel))
   {
     if fuel == 0 || !condition(init) {
       Independence.ReturnIsIndep(init);
     } else {
-      forall init': A ensures Independence.IsIndep(WhileCut(condition, body, init', fuel - 1)) {
+      forall init': A ensures Independence.IsIndep(Monad.WhileCut(condition, body, init', fuel - 1)) {
         WhileCutIsIndep(condition, body, init', fuel - 1);
       }
-      Independence.BindIsIndep(body(init), init' => WhileCut(condition, body, init', fuel - 1));
+      Independence.BindIsIndep(body(init), init' => Monad.WhileCut(condition, body, init', fuel - 1));
     }
   }
 
   lemma WhileIsIndep<A(!new)>(condition: A -> bool, body: A -> Monad.Hurd<A>, init: A)
     requires forall a: A :: Independence.IsIndep(body(a))
-    requires WhileTerminatesAlmostSurely(condition, body)
-    ensures Independence.IsIndep(While(condition, body)(init))
+    requires Monad.WhileTerminatesAlmostSurely(condition, body)
+    ensures Independence.IsIndep(Monad.While(condition, body)(init))
   {
     // To prove this, we need a definition of Independence.IsIndep
     assume {:axiom} false;
@@ -379,9 +169,9 @@ module Loops {
   {
     var reject := (a: A) => !accept(a);
     var body := (a: A) => proposal;
-    forall init: A ensures Independence.IsIndep(While(reject, body)(init)) {
+    forall init: A ensures Independence.IsIndep(Monad.While(reject, body)(init)) {
       WhileIsIndep(reject, body, init);
     }
-    Independence.BindIsIndep(proposal, While(reject, body));
+    Independence.BindIsIndep(proposal, Monad.While(reject, body));
   }
 }
