src/ProbabilisticProgramming/Monad.dfy
@@ -4,8 +4,62 @@
  *******************************************************************************/
 
 module Monad {
+  import Helper
+  import Quantifier
   import Rand
   import Measures
+
+  export
+  provides
+    Helper,
+    Quantifier,
+    Rand,
+    Measures,
+    Hurd,
+    Return,
+    Bind,
+    Coin,
+    While,
+    WhileUnroll,
+    WhileUnroll',
+    Run,
+    LiftInEventSpaceToResultEventSpace,
+    LiftRestInEventSpaceToResultEventSpace
+  reveals
+    Result,
+    Result.Map,
+    Result.Bind,
+    Result.In,
+    Result.Equals,
+    Result.Satisfies,
+    Result.RestIn,
+    Result.RestSatisfies,
+    Values,
+    Rests,
+    ResultEventSpace,
+    boolResultEventSpace,
+    natResultEventSpace,
+    ResultsWithValueIn,
+    ResultsWithRestIn,
+    Composition,
+    Map,
+    Join,
+    WhileCut,
+    WhileCutTerminates,
+    WhileCutTerminatesWithFuel,
+    WhileTerminatesAlmostSurely,
+    LeastFuel
+
+  export MonadInternals
+  extends Monad
+  reveals
+    Hurd,
+    Return,
+    Bind,
+    Coin,
+    While,
+    Run
+
 
   /************
    Definitions
@@ -31,7 +85,7 @@ module Monad {
     function Bind<B>(f: A -> Hurd<B>): Result<B> {
       match this
       case Diverging => Diverging
-      case Result(value, rest) => f(value)(rest)
+      case Result(value, rest) => Run(f(value))(rest)
     }
 
     ghost predicate In(s: iset<A>) {
@@ -84,19 +138,27 @@ module Monad {
   }
 
   // Equation (3.4)
-  function Bind<A,B>(f: Hurd<A>, g: A -> Hurd<B>): Hurd<B> {
+  function Bind<A,B>(f: Hurd<A>, g: A -> Hurd<B>): (m: Hurd<B>)
+    ensures forall s: Rand.Bitstream :: Run(m)(s) == Run(f)(s).Bind(g)
+  {
     (s: Rand.Bitstream) => f(s).Bind(g)
   }
 
   // Equation (2.42)
-  const Coin: Hurd<bool> := s => Result(Rand.Head(s), Rand.Tail(s))
+  function Coin(): Hurd<bool>
+    ensures forall s: Rand.Bitstream :: Run(Coin())(s) == Result(Rand.Head(s), Rand.Tail(s))
+  {
+    s => Result(Rand.Head(s), Rand.Tail(s))
+  }
 
   function Composition<A,B,C>(f: A -> Hurd<B>, g: B -> Hurd<C>): A -> Hurd<C> {
     (a: A) => Bind(f(a), g)
   }
 
   // Equation (3.3)
-  function Return<A>(a: A): Hurd<A> {
+  function Return<A>(a: A): (m: Hurd<A>)
+    ensures forall s: Rand.Bitstream :: Run(m)(s) == Result(a, s)
+  {
     (s: Rand.Bitstream) => Result(a, s)
   }
 
@@ -105,7 +167,69 @@ module Monad {
   }
 
   function Join<A>(ff: Hurd<Hurd<A>>): Hurd<A> {
-    (s: Rand.Bitstream) => ff(s).Bind(f => f)
+    Bind(ff, f => f)
+  }
+
+  function Run<A>(m: Hurd<A>): Rand.Bitstream -> Result<A> {
+    m
+  }
+
+  ghost predicate WhileCutTerminates<A>(condition: A -> bool, body: A -> Hurd<A>, init: A, s: Rand.Bitstream) {
+    exists fuel: nat :: WhileCutTerminatesWithFuel(condition, body, init, s)(fuel)
+  }
+
+  ghost function WhileCutTerminatesWithFuel<A>(condition: A -> bool, body: A -> Hurd<A>, init: A, s: Rand.Bitstream): nat -> bool {
+    (fuel: nat) => !Run(WhileCut(condition, body, init, fuel))(s).Satisfies(condition)
+  }
+
+  // Definition 37
+  function WhileCut<A>(condition: A -> bool, body: A -> Hurd<A>, init: A, fuel: nat): Hurd<A> {
+    if fuel == 0 || !condition(init) then
+      Return(init)
+    else
+      Bind(body(init), (init': A) => WhileCut(condition, body, init', fuel - 1))
+  }
+
+  // Definition of while loops.
+  // This definition is opaque because the details are not very useful.
+  // For proofs, use the lemma `WhileUnroll`.
+  // Equation (3.25), but modified to use `Diverging` instead of HOL's `arb` in case of nontermination
+  opaque ghost function While<A(!new)>(condition: A -> bool, body: A -> Hurd<A>): (loop: A -> Hurd<A>)
+    ensures forall s: Rand.Bitstream, init: A :: !condition(init) ==> Run(loop(init))(s) == Run(Return(init))(s)
+  {
+    var f :=
+      (init: A) =>
+        (s: Rand.Bitstream) =>
+          if WhileCutTerminates(condition, body, init, s)
+          then
+            var fuel := LeastFuel(condition, body, init, s);
+            WhileCut(condition, body, init, fuel)(s)
+          else
+            Diverging;
+    assert forall s: Rand.Bitstream, init: A :: !condition(init) ==> f(init)(s) == Return(init)(s) by {
+      forall s: Rand.Bitstream, init: A ensures !condition(init) ==> f(init)(s) == Return(init)(s) {
+        if !condition(init) {
+          assert WhileCutTerminatesWithFuel(condition, body, init, s)(0);
+        }
+      }
+    }
+    f
+  }
+
+  // Definition 39 / True iff Prob(iset s | While(condition, body, a)(s) terminates) == 1
+  ghost predicate WhileTerminatesAlmostSurely<A(!new)>(condition: A -> bool, body: A -> Hurd<A>) {
+    var p := (init: A) =>
+               (s: Rand.Bitstream) => WhileCutTerminates(condition, body, init, s);
+    forall init :: Quantifier.AlmostSurely(p(init))
+  }
+
+  ghost function LeastFuel<A>(condition: A -> bool, body: A -> Hurd<A>, init: A, s: Rand.Bitstream): (fuel: nat)
+    requires WhileCutTerminates(condition, body, init, s)
+    ensures WhileCutTerminatesWithFuel(condition, body, init, s)(fuel)
+    ensures forall fuel': nat :: WhileCutTerminatesWithFuel(condition, body, init, s)(fuel') ==> fuel <= fuel'
+  {
+    var fuelBound :| WhileCutTerminatesWithFuel(condition, body, init, s)(fuelBound);
+    Helper.Least(WhileCutTerminatesWithFuel(condition, body, init, s), fuelBound)
   }
 
   /*******
@@ -195,6 +319,158 @@ module Monad {
         assert Rests(results) == iset{};
       }
     }
+  }
+
+    lemma LeastFuelUnroll<A>(condition: A -> bool, body: A -> Hurd<A>, init: A, s: Rand.Bitstream, init': A, s': Rand.Bitstream, fuel': nat)
+    requires WhileCutTerminates(condition, body, init', s')
+    requires LeastFuel(condition, body, init', s') == fuel'
+    requires condition(init)
+    requires body(init)(s) == Result(init', s')
+    ensures WhileCutTerminates(condition, body, init, s)
+    ensures LeastFuel(condition, body, init, s) == fuel' + 1
+  {
+    assert WhileCutTerminates(condition, body, init, s) by {
+      WhileCutTerminatesWithFuelUnroll(condition, body, init, s, init', s', fuel');
+    }
+    var fuel := LeastFuel(condition, body, init, s);
+    assert fuel == fuel' + 1 by {
+      WhileCutTerminatesWithFuelUnroll(condition, body, init, s, init', s', fuel');
+      WhileCutTerminatesWithFuelUnroll(condition, body, init, s, init', s', fuel - 1);
+    }
+  }
+
+  lemma WhileCutUnroll<A>(condition: A -> bool, body: A -> Hurd<A>, init: A, s: Rand.Bitstream, init': A, s': Rand.Bitstream, fuel: nat)
+    requires condition(init)
+    requires body(init)(s) == Result(init', s')
+    ensures WhileCut(condition, body, init, fuel + 1)(s) == WhileCut(condition, body, init', fuel)(s')
+  {}
+
+
+  lemma WhileCutTerminatesWithFuelUnroll<A>(condition: A -> bool, body: A -> Hurd<A>, init: A, s: Rand.Bitstream, init': A, s': Rand.Bitstream, fuel: nat)
+    requires condition(init)
+    requires body(init)(s) == Result(init', s')
+    ensures WhileCutTerminatesWithFuel(condition, body, init, s)(fuel + 1) == WhileCutTerminatesWithFuel(condition, body, init', s')(fuel)
+  {}
+
+  lemma WhileCutTerminatesUnroll<A>(condition: A -> bool, body: A -> Hurd<A>, init: A, s: Rand.Bitstream, init': A, s': Rand.Bitstream)
+    requires condition(init)
+    requires body(init)(s) == Result(init', s')
+    ensures WhileCutTerminates(condition, body, init, s) == WhileCutTerminates(condition, body, init', s')
+  {
+    if WhileCutTerminates(condition, body, init, s) {
+      var fuel: nat :| WhileCutTerminatesWithFuel(condition, body, init, s)(fuel);
+      WhileCutTerminatesWithFuelUnroll(condition, body, init, s, init', s', fuel - 1);
+    }
+    if WhileCutTerminates(condition, body, init', s') {
+      var fuel: nat :| WhileCutTerminatesWithFuel(condition, body, init', s')(fuel);
+      WhileCutTerminatesWithFuelUnroll(condition, body, init, s, init', s', fuel);
+    }
+  }
+
+  lemma WhileUnrollIfConditionSatisfied<A>(condition: A -> bool, body: A -> Hurd<A>, init: A, s: Rand.Bitstream, init': A, s': Rand.Bitstream, loop: Result<A>, unrolled: Result<A>)
+    requires WhileCutTerminates(condition, body, init, s)
+    requires condition(init)
+    requires body(init)(s) == Result(init', s')
+    requires loop == While(condition, body)(init)(s)
+    requires unrolled == While(condition, body)(init')(s')
+    ensures loop == unrolled
+  {
+    var fuel: nat := LeastFuel(condition, body, init, s);
+    assert fuel >= 1;
+    var fuel': nat := fuel - 1;
+    assert WhileCutTerminatesWithFuel(condition, body, init', s')(fuel');
+    assert WhileCutTerminates(condition, body, init', s');
+    var minFuel: nat := LeastFuel(condition, body, init', s');
+    assert minFuel == fuel' by {
+      LeastFuelUnroll(condition, body, init, s, init', s', minFuel);
+    }
+    assert loop == unrolled by {
+      calc {
+        loop;
+        { reveal While(); }
+        WhileCut(condition, body, init, fuel)(s);
+        { WhileCutUnroll(condition, body, init, s, init', s', fuel'); }
+        WhileCut(condition, body, init', fuel')(s');
+        { reveal While(); }
+        unrolled;
+      }
+    }
+  }
+
+  lemma WhileUnrollIfTerminates<A(!new)>(condition: A -> bool, body: A -> Hurd<A>, init: A, s: Rand.Bitstream, fuel: nat, loop: Result<A>, unrolled: Result<A>)
+    requires WhileCutTerminates(condition, body, init, s)
+    requires fuel == LeastFuel(condition, body, init, s)
+    requires loop == While(condition, body)(init)(s)
+    requires unrolled == (if condition(init) then Bind(body(init), While(condition, body)) else Return(init))(s)
+    ensures loop == unrolled
+  {
+    if condition(init) {
+      assert fuel >= 1;
+      match body(init)(s)
+      case Diverging =>
+        calc {
+          loop;
+          { reveal While(); }
+          WhileCut(condition, body, init, fuel)(s);
+          Diverging;
+          unrolled;
+        }
+      case Result(init', s') =>
+        calc {
+          loop;
+          { WhileUnrollIfConditionSatisfied(condition, body, init, s, init', s', loop, unrolled); }
+          While(condition, body)(init')(s');
+          unrolled;
+        }
+    } else {
+      calc {
+        loop;
+        Result(init, s);
+        unrolled;
+      }
+    }
+  }
+
+  lemma WhileUnrollIfDiverges<A>(condition: A -> bool, body: A -> Hurd<A>, init: A, s: Rand.Bitstream, loop: Result<A>, unrolled: Result<A>)
+    requires !WhileCutTerminates(condition, body, init, s)
+    requires loop == While(condition, body)(init)(s)
+    requires unrolled == (if condition(init) then Bind(body(init), While(condition, body)) else Return(init))(s)
+    ensures loop == unrolled == Diverging
+  {
+    reveal While();
+    match body(init)(s)
+    case Diverging =>
+      assert unrolled == Diverging;
+    case Result(init', s') =>
+      assert !WhileCutTerminates(condition, body, init', s') by {
+        WhileCutTerminatesUnroll(condition, body, init, s, init', s');
+      }
+  }
+
+  // Theorem 38
+  lemma WhileUnroll<A(!new)>(condition: A -> bool, body: A -> Hurd<A>, init: A, s: Rand.Bitstream)
+    requires WhileTerminatesAlmostSurely(condition, body)
+    ensures Run(While(condition, body)(init))(s) == Run(if condition(init) then Bind(body(init), While(condition, body)) else Return(init))(s)
+  {
+    var loop := While(condition, body)(init)(s);
+    var unrolled := (if condition(init) then Bind(body(init), While(condition, body)) else Return(init))(s);
+    assert loop == unrolled by {
+      if WhileCutTerminates(condition, body, init, s) {
+        var fuel: nat := LeastFuel(condition, body, init, s);
+        WhileUnrollIfTerminates(condition, body, init, s, fuel, loop, unrolled);
+      } else {
+        WhileUnrollIfDiverges(condition, body, init, s, loop, unrolled);
+      }
+    }
+  }
+
+  lemma WhileUnroll'<A(!new)>(condition: A -> bool, body: A -> Hurd<A>, init: A, s: Rand.Bitstream, w: A -> Hurd<A>, i: Hurd<A>)
+    requires WhileTerminatesAlmostSurely(condition, body)
+    requires w == While(condition, body)
+    requires i == if condition(init) then Bind(body(init), While(condition, body)) else Return(init)
+    ensures Run(w(init))(s) == Run(i)(s)
+  {
+    WhileUnroll(condition, body, init, s);
   }
 }
 
